Example with tagged pointers.

examples/tagged_ptr.c
@@ -1,0 +1,59 @@
+#include <stddef.h>
+#include <stdint.h>
+#include <refinedc.h>
+
+#define TAG_SIZE 3
+#define TAG_MOD  (1 << TAG_SIZE)
+#define TAG_MASK (TAG_MOD - 1)
+
+typedef unsigned char tag_t;
+
+//@rc::inlined Notation TAG_MOD := (8%nat) (only parsing).
+
+[[rc::parameters("r: {loc * Z}", "ty : type", "v : val")]]
+[[rc::args("value<void*, v>")]]
+[[rc::requires("v : r @ tagged_ptr<Own, TAG_MOD, ty>")]]
+[[rc::returns("{r.2} @ int<u8>")]]
+[[rc::ensures("{0 ≤ r.2 < TAG_MOD}")]]
+[[rc::ensures("v : r @ tagged_ptr<Own, TAG_MOD, ty>")]]
+tag_t tag_of(void* p){
+  return ((uintptr_t) p) % TAG_MOD;
+}
+
+[[rc::parameters("r: {loc * Z}", "t: Z", "ty: type")]]
+[[rc::args("r @ tagged_ptr<Own, TAG_MOD, ty>", "t @ int<u8>")]]
+[[rc::requires("{0 ≤ t < TAG_MOD}")]]
+[[rc::returns("{(r.1, t)} @ tagged_ptr<Own, TAG_MOD, ty>")]]
+void* tag(void* p, tag_t t){
+  tag_t old_t = tag_of(p);
+  return rc_copy_alloc_id((void*) ((uintptr_t) p - old_t + t), p);
+}
+
+[[rc::parameters("r: {loc * Z}", "ty: type")]]
+[[rc::args("r @ tagged_ptr<Own, TAG_MOD, ty>")]]
+[[rc::returns("{r.1} @ &own<ty>")]]
+void* untag(void* p){
+  uintptr_t i = (uintptr_t) p;
+  return rc_copy_alloc_id((void*) (i - i % TAG_MOD), p);
+}
+
+[[rc::returns("{0} @ int<size_t>")]]
+size_t test(){
+  size_t x = 0;
+
+  void *tp = tag(&x, 1);
+  assert(tag_of(tp) == 1);
+
+  size_t *px = (size_t *) untag(tp);
+  return *px;
+}
+
+[[rc::parameters("l: loc", "beta: own_state", "n: Z")]]
+[[rc::args("l @ &frac<beta, n @ int<i32>>")]]
+[[rc::returns("{bool_decide (l `aligned_to` 8%nat)} @ boolean<i32>")]]
+[[rc::ensures("frac beta l : n @ int<i32>")]]
+[[rc::tactics("all: unfold aligned_to in *; split; solve_goal.")]]
+int is_aligned(void* p){
+  uintptr_t i = (uintptr_t) p;
+  return i % TAG_MOD == 0;
+}
