examples/proofs/tagged_ptr/generated_code.v
@@ -1,0 +1,198 @@
+From refinedc.lang Require Export notation.
+From refinedc.lang Require Import tactics.
+From refinedc.typing Require Import annotations.
+Set Default Proof Using "Type".
+
+(* Generated from [examples/tagged_ptr.c]. *)
+Section code.
+  Definition file_0 : string := "examples/tagged_ptr.c".
+  Definition loc_2 : location_info := LocationInfo file_0 20 2 20 36.
+  Definition loc_3 : location_info := LocationInfo file_0 20 9 20 35.
+  Definition loc_4 : location_info := LocationInfo file_0 20 9 20 24.
+  Definition loc_5 : location_info := LocationInfo file_0 20 22 20 23.
+  Definition loc_6 : location_info := LocationInfo file_0 20 22 20 23.
+  Definition loc_7 : location_info := LocationInfo file_0 20 27 20 35.
+  Definition loc_8 : location_info := LocationInfo file_0 20 28 20 29.
+  Definition loc_9 : location_info := LocationInfo file_0 20 33 20 34.
+  Definition loc_12 : location_info := LocationInfo file_0 28 2 28 26.
+  Definition loc_13 : location_info := LocationInfo file_0 29 2 29 139.
+  Definition loc_14 : location_info := LocationInfo file_0 29 9 29 138.
+  Definition loc_15 : location_info := LocationInfo file_0 29 35 29 38.
+  Definition loc_16 : location_info := LocationInfo file_0 29 35 29 38.
+  Definition loc_17 : location_info := LocationInfo file_0 29 40 29 77.
+  Definition loc_18 : location_info := LocationInfo file_0 29 49 29 76.
+  Definition loc_19 : location_info := LocationInfo file_0 29 50 29 71.
+  Definition loc_20 : location_info := LocationInfo file_0 29 50 29 63.
+  Definition loc_21 : location_info := LocationInfo file_0 29 62 29 63.
+  Definition loc_22 : location_info := LocationInfo file_0 29 62 29 63.
+  Definition loc_23 : location_info := LocationInfo file_0 29 66 29 71.
+  Definition loc_24 : location_info := LocationInfo file_0 29 66 29 71.
+  Definition loc_25 : location_info := LocationInfo file_0 29 74 29 75.
+  Definition loc_26 : location_info := LocationInfo file_0 29 74 29 75.
+  Definition loc_27 : location_info := LocationInfo file_0 28 16 28 25.
+  Definition loc_28 : location_info := LocationInfo file_0 28 16 28 22.
+  Definition loc_29 : location_info := LocationInfo file_0 28 16 28 22.
+  Definition loc_30 : location_info := LocationInfo file_0 28 23 28 24.
+  Definition loc_31 : location_info := LocationInfo file_0 28 23 28 24.
+  Definition loc_36 : location_info := LocationInfo file_0 36 2 36 30.
+  Definition loc_37 : location_info := LocationInfo file_0 37 2 37 121.
+  Definition loc_38 : location_info := LocationInfo file_0 37 9 37 120.
+  Definition loc_39 : location_info := LocationInfo file_0 37 35 37 38.
+  Definition loc_40 : location_info := LocationInfo file_0 37 35 37 38.
+  Definition loc_41 : location_info := LocationInfo file_0 37 40 37 68.
+  Definition loc_42 : location_info := LocationInfo file_0 37 49 37 67.
+  Definition loc_43 : location_info := LocationInfo file_0 37 50 37 51.
+  Definition loc_44 : location_info := LocationInfo file_0 37 50 37 51.
+  Definition loc_45 : location_info := LocationInfo file_0 37 54 37 66.
+  Definition loc_46 : location_info := LocationInfo file_0 37 54 37 55.
+  Definition loc_47 : location_info := LocationInfo file_0 37 54 37 55.
+  Definition loc_48 : location_info := LocationInfo file_0 37 58 37 66.
+  Definition loc_49 : location_info := LocationInfo file_0 37 59 37 60.
+  Definition loc_50 : location_info := LocationInfo file_0 37 64 37 65.
+  Definition loc_51 : location_info := LocationInfo file_0 36 16 36 29.
+  Definition loc_52 : location_info := LocationInfo file_0 36 28 36 29.
+  Definition loc_53 : location_info := LocationInfo file_0 36 28 36 29.
+  Definition loc_58 : location_info := LocationInfo file_0 42 2 42 15.
+  Definition loc_59 : location_info := LocationInfo file_0 44 2 44 24.
+  Definition loc_60 : location_info := LocationInfo file_0 45 2 45 26.
+  Definition loc_61 : location_info := LocationInfo file_0 47 2 47 36.
+  Definition loc_62 : location_info := LocationInfo file_0 48 2 48 13.
+  Definition loc_63 : location_info := LocationInfo file_0 48 9 48 12.
+  Definition loc_64 : location_info := LocationInfo file_0 48 9 48 12.
+  Definition loc_65 : location_info := LocationInfo file_0 48 10 48 12.
+  Definition loc_66 : location_info := LocationInfo file_0 48 10 48 12.
+  Definition loc_67 : location_info := LocationInfo file_0 47 15 47 35.
+  Definition loc_68 : location_info := LocationInfo file_0 47 26 47 35.
+  Definition loc_69 : location_info := LocationInfo file_0 47 26 47 31.
+  Definition loc_70 : location_info := LocationInfo file_0 47 26 47 31.
+  Definition loc_71 : location_info := LocationInfo file_0 47 32 47 34.
+  Definition loc_72 : location_info := LocationInfo file_0 47 32 47 34.
+  Definition loc_75 : location_info := LocationInfo file_0 45 9 45 24.
+  Definition loc_76 : location_info := LocationInfo file_0 45 9 45 19.
+  Definition loc_77 : location_info := LocationInfo file_0 45 9 45 15.
+  Definition loc_78 : location_info := LocationInfo file_0 45 9 45 15.
+  Definition loc_79 : location_info := LocationInfo file_0 45 16 45 18.
+  Definition loc_80 : location_info := LocationInfo file_0 45 16 45 18.
+  Definition loc_81 : location_info := LocationInfo file_0 45 23 45 24.
+  Definition loc_82 : location_info := LocationInfo file_0 44 13 44 23.
+  Definition loc_83 : location_info := LocationInfo file_0 44 13 44 16.
+  Definition loc_84 : location_info := LocationInfo file_0 44 13 44 16.
+  Definition loc_85 : location_info := LocationInfo file_0 44 17 44 19.
+  Definition loc_86 : location_info := LocationInfo file_0 44 18 44 19.
+  Definition loc_87 : location_info := LocationInfo file_0 44 21 44 22.
+  Definition loc_90 : location_info := LocationInfo file_0 42 13 42 14.
+  Definition loc_95 : location_info := LocationInfo file_0 57 2 57 30.
+  Definition loc_96 : location_info := LocationInfo file_0 58 2 58 27.
+  Definition loc_97 : location_info := LocationInfo file_0 58 9 58 26.
+  Definition loc_98 : location_info := LocationInfo file_0 58 9 58 21.
+  Definition loc_99 : location_info := LocationInfo file_0 58 9 58 10.
+  Definition loc_100 : location_info := LocationInfo file_0 58 9 58 10.
+  Definition loc_101 : location_info := LocationInfo file_0 58 13 58 21.
+  Definition loc_102 : location_info := LocationInfo file_0 58 14 58 15.
+  Definition loc_103 : location_info := LocationInfo file_0 58 19 58 20.
+  Definition loc_104 : location_info := LocationInfo file_0 58 25 58 26.
+  Definition loc_105 : location_info := LocationInfo file_0 57 16 57 29.
+  Definition loc_106 : location_info := LocationInfo file_0 57 28 57 29.
+  Definition loc_107 : location_info := LocationInfo file_0 57 28 57 29.
+
+  (* Definition of function [tag_of]. *)
+  Definition impl_tag_of : function := {|
+    f_args := [
+      ("p", void*)
+    ];
+    f_local_vars := [
+    ];
+    f_init := "#0";
+    f_code := (
+      <[ "#0" :=
+        locinfo: loc_2 ;
+        Return (LocInfoE loc_3 (UnOp (CastOp $ IntOp u8) (IntOp uintptr_t) (LocInfoE loc_3 ((LocInfoE loc_4 (UnOp (CastOp $ IntOp uintptr_t) (PtrOp) (LocInfoE loc_5 (use{void*} (LocInfoE loc_6 ("p")))))) %{IntOp uintptr_t, IntOp uintptr_t} (LocInfoE loc_7 (UnOp (CastOp $ IntOp uintptr_t) (IntOp i32) (LocInfoE loc_7 ((LocInfoE loc_8 (i2v 1 i32)) <<{IntOp i32, IntOp i32} (LocInfoE loc_9 (i2v 3 i32))))))))))
+      ]> $∅
+    )%E
+  |}.
+
+  (* Definition of function [tag]. *)
+  Definition impl_tag (global_tag_of : loc): function := {|
+    f_args := [
+      ("p", void*);
+      ("t", it_layout u8)
+    ];
+    f_local_vars := [
+      ("old_t", it_layout u8)
+    ];
+    f_init := "#0";
+    f_code := (
+      <[ "#0" :=
+        "old_t" <-{ it_layout u8 }
+          LocInfoE loc_27 (Call (LocInfoE loc_29 (global_tag_of)) [@{expr} LocInfoE loc_30 (use{void*} (LocInfoE loc_31 ("p"))) ]) ;
+        locinfo: loc_13 ;
+        Return (LocInfoE loc_14 (CopyAllocId (PtrOp) (LocInfoE loc_17 (UnOp (CastOp $ PtrOp) (IntOp uintptr_t) (LocInfoE loc_18 ((LocInfoE loc_19 ((LocInfoE loc_20 (UnOp (CastOp $ IntOp uintptr_t) (PtrOp) (LocInfoE loc_21 (use{void*} (LocInfoE loc_22 ("p")))))) -{IntOp uintptr_t, IntOp uintptr_t} (LocInfoE loc_23 (UnOp (CastOp $ IntOp uintptr_t) (IntOp u8) (LocInfoE loc_23 (use{it_layout u8} (LocInfoE loc_24 ("old_t")))))))) +{IntOp uintptr_t, IntOp uintptr_t} (LocInfoE loc_25 (UnOp (CastOp $ IntOp uintptr_t) (IntOp u8) (LocInfoE loc_25 (use{it_layout u8} (LocInfoE loc_26 ("t")))))))))) (LocInfoE loc_15 (use{void*} (LocInfoE loc_16 ("p"))))))
+      ]> $∅
+    )%E
+  |}.
+
+  (* Definition of function [untag]. *)
+  Definition impl_untag : function := {|
+    f_args := [
+      ("p", void*)
+    ];
+    f_local_vars := [
+      ("i", it_layout uintptr_t)
+    ];
+    f_init := "#0";
+    f_code := (
+      <[ "#0" :=
+        "i" <-{ it_layout uintptr_t }
+          LocInfoE loc_51 (UnOp (CastOp $ IntOp uintptr_t) (PtrOp) (LocInfoE loc_52 (use{void*} (LocInfoE loc_53 ("p"))))) ;
+        locinfo: loc_37 ;
+        Return (LocInfoE loc_38 (CopyAllocId (PtrOp) (LocInfoE loc_41 (UnOp (CastOp $ PtrOp) (IntOp uintptr_t) (LocInfoE loc_42 ((LocInfoE loc_43 (use{it_layout uintptr_t} (LocInfoE loc_44 ("i")))) -{IntOp uintptr_t, IntOp uintptr_t} (LocInfoE loc_45 ((LocInfoE loc_46 (use{it_layout uintptr_t} (LocInfoE loc_47 ("i")))) %{IntOp uintptr_t, IntOp uintptr_t} (LocInfoE loc_48 (UnOp (CastOp $ IntOp uintptr_t) (IntOp i32) (LocInfoE loc_48 ((LocInfoE loc_49 (i2v 1 i32)) <<{IntOp i32, IntOp i32} (LocInfoE loc_50 (i2v 3 i32)))))))))))) (LocInfoE loc_39 (use{void*} (LocInfoE loc_40 ("p"))))))
+      ]> $∅
+    )%E
+  |}.
+
+  (* Definition of function [test]. *)
+  Definition impl_test (global_tag global_tag_of global_untag : loc): function := {|
+    f_args := [
+    ];
+    f_local_vars := [
+      ("tp", void*);
+      ("x", it_layout size_t);
+      ("px", void*)
+    ];
+    f_init := "#0";
+    f_code := (
+      <[ "#0" :=
+        "x" <-{ it_layout size_t }
+          LocInfoE loc_90 (UnOp (CastOp $ IntOp size_t) (IntOp i32) (LocInfoE loc_90 (i2v 0 i32))) ;
+        "tp" <-{ void* }
+          LocInfoE loc_82 (Call (LocInfoE loc_84 (global_tag)) [@{expr} LocInfoE loc_85 (&(LocInfoE loc_86 ("x"))) ;
+          LocInfoE loc_87 (UnOp (CastOp $ IntOp u8) (IntOp i32) (LocInfoE loc_87 (i2v 1 i32))) ]) ;
+        locinfo: loc_60 ;
+        assert: (LocInfoE loc_75 (UnOp (CastOp $ IntOp bool_it) (IntOp i32) (LocInfoE loc_75 ((LocInfoE loc_76 (UnOp (CastOp $ IntOp i32) (IntOp u8) (LocInfoE loc_76 (Call (LocInfoE loc_78 (global_tag_of)) [@{expr} LocInfoE loc_79 (use{void*} (LocInfoE loc_80 ("tp"))) ])))) ={IntOp i32, IntOp i32} (LocInfoE loc_81 (i2v 1 i32)))))) ;
+        "px" <-{ void* }
+          LocInfoE loc_67 (UnOp (CastOp $ PtrOp) (PtrOp) (LocInfoE loc_68 (Call (LocInfoE loc_70 (global_untag)) [@{expr} LocInfoE loc_71 (use{void*} (LocInfoE loc_72 ("tp"))) ]))) ;
+        locinfo: loc_62 ;
+        Return (LocInfoE loc_63 (use{it_layout size_t} (LocInfoE loc_65 (!{void*} (LocInfoE loc_66 ("px"))))))
+      ]> $∅
+    )%E
+  |}.
+
+  (* Definition of function [is_aligned]. *)
+  Definition impl_is_aligned : function := {|
+    f_args := [
+      ("p", void*)
+    ];
+    f_local_vars := [
+      ("i", it_layout uintptr_t)
+    ];
+    f_init := "#0";
+    f_code := (
+      <[ "#0" :=
+        "i" <-{ it_layout uintptr_t }
+          LocInfoE loc_105 (UnOp (CastOp $ IntOp uintptr_t) (PtrOp) (LocInfoE loc_106 (use{void*} (LocInfoE loc_107 ("p"))))) ;
+        locinfo: loc_96 ;
+        Return (LocInfoE loc_97 ((LocInfoE loc_98 ((LocInfoE loc_99 (use{it_layout uintptr_t} (LocInfoE loc_100 ("i")))) %{IntOp uintptr_t, IntOp uintptr_t} (LocInfoE loc_101 (UnOp (CastOp $ IntOp uintptr_t) (IntOp i32) (LocInfoE loc_101 ((LocInfoE loc_102 (i2v 1 i32)) <<{IntOp i32, IntOp i32} (LocInfoE loc_103 (i2v 3 i32)))))))) ={IntOp uintptr_t, IntOp uintptr_t} (LocInfoE loc_104 (UnOp (CastOp $ IntOp uintptr_t) (IntOp i32) (LocInfoE loc_104 (i2v 0 i32))))))
+      ]> $∅
+    )%E
+  |}.
+End code.
