examples/proofs/tagged_ptr/generated_proof_tag.v
@@ -1,0 +1,27 @@
+From refinedc.typing Require Import typing.
+From refinedc.examples.tagged_ptr Require Import generated_code.
+From refinedc.examples.tagged_ptr Require Import generated_spec.
+Set Default Proof Using "Type".
+
+(* Generated from [examples/tagged_ptr.c]. *)
+Section proof_tag.
+  Context `{!typeG Σ} `{!globalG Σ}.
+
+  (* Typing proof for [tag]. *)
+  Lemma type_tag (global_tag_of : loc) :
+    global_tag_of ◁ᵥ global_tag_of @ function_ptr type_of_tag_of -∗
+    typed_function (impl_tag global_tag_of) type_of_tag.
+  Proof.
+    Open Scope printing_sugar.
+    start_function "tag" ([[r t] ty]) => arg_p arg_t local_old_t.
+    split_blocks ((
+      ∅
+    )%I : gmap label (iProp Σ)) ((
+      ∅
+    )%I : gmap label (iProp Σ)).
+    - repeat liRStep; liShow.
+      all: print_typesystem_goal "tag" "#0".
+    Unshelve. all: sidecond_hook; prepare_sideconditions; normalize_and_simpl_goal; try solve_goal; unsolved_sidecond_hook.
+    all: print_sidecondition_goal "tag".
+  Qed.
+End proof_tag.
