examples/proofs/tagged_ptr/generated_spec.v
@@ -1,0 +1,38 @@
+From refinedc.typing Require Import typing.
+From refinedc.examples.tagged_ptr Require Import generated_code.
+Set Default Proof Using "Type".
+
+(* Generated from [examples/tagged_ptr.c]. *)
+Section spec.
+  Context `{!typeG Σ} `{!globalG Σ}.
+
+  (* Inlined code. *)
+
+  Notation TAG_MOD := (8%nat) (only parsing).
+
+  (* Type definitions. *)
+
+  (* Specifications for function [tag_of]. *)
+  Definition type_of_tag_of :=
+    fn(∀ (r, ty, v) : (loc * Z) * type * val; (value (void*) (v)); (v ◁ᵥ (r @ (tagged_ptr (Own) (TAG_MOD) (ty)))))
+      → ∃ () : (), ((r.2) @ (int (u8))); ⌜0 ≤ r.2 < TAG_MOD⌝ ∗ (v ◁ᵥ (r @ (tagged_ptr (Own) (TAG_MOD) (ty)))).
+
+  (* Specifications for function [tag]. *)
+  Definition type_of_tag :=
+    fn(∀ (r, t, ty) : (loc * Z) * Z * type; (r @ (tagged_ptr (Own) (TAG_MOD) (ty))), (t @ (int (u8))); ⌜0 ≤ t < TAG_MOD⌝)
+      → ∃ () : (), (((r.1, t)) @ (tagged_ptr (Own) (TAG_MOD) (ty))); True.
+
+  (* Specifications for function [untag]. *)
+  Definition type_of_untag :=
+    fn(∀ (r, ty) : (loc * Z) * type; (r @ (tagged_ptr (Own) (TAG_MOD) (ty))); True)
+      → ∃ () : (), ((r.1) @ (&own (ty))); True.
+
+  (* Specifications for function [test]. *)
+  Definition type_of_test :=
+    fn(∀ () : (); True) → ∃ () : (), ((0) @ (int (size_t))); True.
+
+  (* Specifications for function [is_aligned]. *)
+  Definition type_of_is_aligned :=
+    fn(∀ (l, beta, n) : loc * own_state * Z; (l @ (&frac{beta} (n @ (int (i32))))); True)
+      → ∃ () : (), ((bool_decide (l `aligned_to` 8%nat)) @ (boolean (i32))); (l ◁ₗ{beta} (n @ (int (i32)))).
+End spec.
