theories/lang/loc.v
@@ -155,3 +155,6 @@ Proof.
   unfold aligned_to. destruct l => /= ??. apply: Z.divide_add_cancel_r => //.
   apply: (Zdivide_mult_l _ n1). by rewrite Z.mul_comm -Nat2Z.inj_mul.
 Qed.
+
+Instance aligned_to_dec l n : Decision (l `aligned_to` n).
+Proof. apply Znumtheory.Zdivide_dec. Qed.
