theories/typing/tagged_ptr.v
@@ -1,0 +1,117 @@
+From refinedc.typing Require Export type.
+From refinedc.typing Require Import programs own intptr.
+Set Default Proof Using "Type".
+
+Section tagged_ptr.
+  Context `{!typeG Σ}.
+
+  Program Definition tagged_ptr_type (β : own_state) (align : nat) (ty : type) (r : loc * Z) : type := {|
+    ty_own β' l :=
+      ⌜l `has_layout_loc` void*⌝ ∗
+      ⌜r.1 `aligned_to` align⌝ ∗
+      ⌜0 ≤ r.2 < align⌝ ∗
+      l ↦[β'] (r.1 +ₗ r.2) ∗
+      loc_in_bounds r.1 align ∗
+      r.1 ◁ₗ{own_state_min β' β} ty;
+  |}%I.
+  Next Obligation.
+    iIntros (β ??????) "($&$&$&Hl&$&H)". rewrite left_id.
+    iMod (heap_mapsto_own_state_share with "Hl") as "$".
+    destruct β => //=. by iApply ty_share.
+  Qed.
+  Global Instance tagged_ptr_type_ne n : Proper ((=) ==> (dist n) ==> (=) ==> (=) ==> (dist n)) tagged_ptr_type.
+  Proof. solve_type_proper. Qed.
+  Global Instance tagged_ptr_type_proper : Proper ((=) ==> (≡) ==> (=) ==> (=) ==> (≡)) tagged_ptr_type.
+  Proof. solve_type_proper. Qed.
+
+  Program Definition tagged_ptr (β : own_state) (align : nat) (ty : type) : rtype := {|
+    rty_type := loc * Z;
+    rty := tagged_ptr_type β align ty;
+  |}%I.
+
+  Global Program Instance rmovable_tagged_ptr β align ty : RMovable (tagged_ptr β align ty) := {|
+    rmovable r := {|
+      ty_layout := void*;
+      ty_own_val v :=
+        ⌜v = val_of_loc (r.1 +ₗ r.2)⌝ ∗
+        ⌜r.1 `aligned_to` align⌝ ∗
+        ⌜0 ≤ r.2 < align⌝ ∗
+        loc_in_bounds r.1 align ∗
+        r.1 ◁ₗ{β} ty;
+    |}
+  |}%I.
+  Next Obligation. iIntros (?????) "($&_)". Qed.
+  Next Obligation. iIntros (?????) "(->&_)". done. Qed.
+  Next Obligation. iIntros (?????) "(%&%&%&?&?)". rewrite left_id. eauto with iFrame. Qed.
+  Next Obligation. iIntros (???????) "? (->&%&%&?)". iFrame. rewrite left_id. eauto with iFrame. Qed.
+  Next Obligation. done. Qed.
+
+  Global Instance tagged_ptr_loc_in_bounds r ty align β1 β2 :
+    LocInBounds (r @ tagged_ptr β1 align ty) β2 bytes_per_addr.
+  Proof.
+    constructor. iIntros (?) "(_&_&_&Hl&_)".
+    iDestruct (heap_mapsto_own_state_loc_in_bounds with "Hl") as "Hb".
+    iApply loc_in_bounds_shorten; last done. by rewrite /val_of_loc.
+  Qed.
+
+  Global Instance tagged_ptr_related_to_frac_ptr v r β n ty:
+     RelatedTo (v ◁ᵥ r @ tagged_ptr β n ty)%I | 1 :=
+     {| rt_fic := FindValOrLoc v r.1 |}.
+
+  Lemma subsume_tagged_ptr v r1 r2 n1 n2 β1 β2 ty1 ty2 T:
+    (⌜r1 = r2⌝ ∗ ⌜n1 = n2⌝ ∗ ⌜β1 = β2⌝ ∗ subsume (r1.1 ◁ₗ{β1} ty1) (r2.1 ◁ₗ{β2} ty2) T) -∗
+    subsume (v ◁ᵥ r1 @ tagged_ptr β1 n1 ty1) (v ◁ᵥ r2 @ tagged_ptr β2 n2 ty2) T.
+  Proof.
+    iIntros "(->&->&->&HT) ($&$&$&$&?)". by iApply "HT".
+  Qed.
+  Global Instance subsume_tagged_ptr_inst v r1 r2 n1 n2 β1 β2 ty1 ty2:
+    SubsumeVal v (r1 @ tagged_ptr β1 n1 ty1) (r2 @ tagged_ptr β2 n2 ty2) :=
+    λ T, i2p (subsume_tagged_ptr v r1 r2 n1 n2 β1 β2 ty1 ty2 T).
+
+  Lemma subsume_frac_ptr_tagged_ptr l β (v : val) r n ty1 ty2 m T `{!LearnAlignment β ty1 m}:
+    (⌜if m is Some m' then l `aligned_to` m' else True⌝ -∗
+      ⌜l = r.1⌝ ∗ ⌜v = r.1 +ₗ r.2⌝ ∗ ⌜l `aligned_to` n⌝ ∗ ⌜0 ≤ r.2 < n⌝ ∗
+     ((l ◁ₗ{β} ty1 -∗ loc_in_bounds l n ∗ True) ∧ subsume (l ◁ₗ{β} ty1) (l ◁ₗ{β} ty2) T)) -∗
+    subsume (l ◁ₗ{β} ty1) (v ◁ᵥ r @ tagged_ptr β n ty2) T.
+  Proof.
+    iIntros "HT Hl".
+    iDestruct (learnalign_learn with "Hl") as %?.
+    iDestruct ("HT" with "[//]") as "(->&->&%&%&HT)".
+    iAssert (loc_in_bounds r.1 n) as "#Hlib".
+    { iDestruct "HT" as "[HT _]". iDestruct ("HT" with "Hl") as "[$ _]". }
+    iDestruct "HT" as "[_ HT]". iDestruct ("HT" with "Hl") as "[$ $]". by iFrame "Hlib".
+  Qed.
+  Global Instance subsume_frac_ptr_tagged_ptr_inst l β v r n ty1 ty2 m `{!LearnAlignment β ty1 m}:
+    Subsume (l ◁ₗ{β} ty1)%I (v ◁ᵥ r @ tagged_ptr β n ty2)%I :=
+    λ T, i2p (subsume_frac_ptr_tagged_ptr l β v r n ty1 ty2 m T).
+
+  Lemma type_cast_tagged_ptr_intptr_val (v : val) (r : loc * Z) β (align : nat) it ty T:
+    (
+        ⌜v = r.1 +ₗ r.2⌝ -∗
+        ⌜aligned_to r.1 align⌝ -∗
+        ⌜0 ≤ r.2 < align⌝ -∗
+        ⌜min_alloc_start ≤ r.1.2 ∧ r.1.2 + align ≤ max_alloc_end⌝ -∗
+        loc_in_bounds r.1 align -∗
+        r.1 ◁ₗ{β} ty -∗
+        ⌜(r.1.2 + r.2)%Z ∈ it⌝ ∗ T (val_of_loc_n (bytes_per_int it) (r.1 +ₗ r.2)) (t2mt ((r.1 +ₗ r.2) @ intptr it))
+    ) -∗
+    typed_un_op v (v ◁ᵥ r @ tagged_ptr β align ty) (CastOp (IntOp it)) PtrOp T.
+  Proof.
+    iIntros "HT (->&%&%&Hlib&Hp)" (Φ) "HΦ".
+    iDestruct (loc_in_bounds_ptr_in_range with "Hlib") as %Hrange.
+    iDestruct ("HT" with "[//] [//] [//] [//] [$] [$]") as (Hr) "HT".
+    iApply wp_cast_ptr_int => //=; first by rewrite val_to_of_loc.
+    { by rewrite bool_decide_true. }
+    iApply ("HΦ" with "[] HT").
+    iPureIntro. by apply val_to_loc_weak_val_of_loc_n.
+  Qed.
+  Global Instance type_cast_tagged_ptr_intptr_val_inst (v : val) (r : loc * Z) β (align : nat) it ty:
+    TypedUnOp v (v ◁ᵥ r @ tagged_ptr β align ty)%I (CastOp (IntOp it)) PtrOp :=
+    λ T, i2p (type_cast_tagged_ptr_intptr_val v r β align it ty T).
+
+End tagged_ptr.
+Typeclasses Opaque tagged_ptr_type.
+
+Notation "tagged_ptr< β , align , ty >" :=
+  (tagged_ptr β align ty)
+  (only printing, format "'tagged_ptr<' β , align , ty '>'") : printing_sugar.
